assigned some names to continuation variables.
These variables are generated during during CPS conversion,
unlike other variables whose names come from the user.
Although, the proofs about CPS conversion
are not explicitly parametric over the names for continuation vars,
changing these names (in L4a_to_L5.v) should not break any proof.

theories/L4_deBruijn/L4a_to_L5.v
@@ -118,7 +118,7 @@ Require Import Coq.Strings.Ascii.
 
 Require Import  ExtLib.Data.String.
 
-Definition sconString (d: dcon) : string :=
+Definition dconString (d: dcon) : string :=
 match fst d with
 | mkInd s n => terms.flatten [nat2string10 (N.to_nat (snd d))
     ; ":"; nat2string10 n; ":"; s]
@@ -131,13 +131,13 @@ Definition L4OpidString (l : L4Opid) : string :=
   match l with
   | NLambda    => "λ"
   | NFix _ _ => "fix"
-  | NDCon d _ => sconString d
+  | NDCon d _ => dconString d
   | NApply     => "ap"
 (*  | NProj _ => [0] *)
   | NLet => "let"
   | NMatch numargsInBranches => 
       let ld := map fst numargsInBranches in
-      terms.flatten ["match |";terms.flattenDelim " " (map sconString ld);"|"]
+      terms.flatten ["match |";terms.flattenDelim " " (map dconString ld);"|"]
   end.
 
 
@@ -207,14 +207,14 @@ Definition L5OpidString (l : L5Opid) : string :=
   | CLambda    => "λ"
   | CKLambda    => "λ→" 
   | CFix _ _ => "fix"
-  | CDCon d _ => sconString d
+  | CDCon d _ => dconString d
   | CRet     => "ret"
 (*  | NProj _ => [0] *)
   | CCall => "call"
   | CHalt => "halt"
   | CMatch numargsInBranches => 
       let ld := map fst numargsInBranches in
-      terms.flatten ["match |";terms.flattenDelim " " (map sconString ld);"|"]
+      terms.flatten ["match |";terms.flattenDelim " " (map dconString ld);"|"]
   end.
 
 
@@ -231,13 +231,16 @@ Instance CPSGenericTermSig : GenericTermSig L5Opid:=
 |}.
 
 
+Require Import L4.varInterface.
 
 Section VarsOf2Class.
+
 
 (* see the file SquiggleEq.varImplPeano for an instantiation of NVar *)
 Context {NVar} {deqnvar : Deq NVar} 
 {varcl freshv} 
-  {varclass: @VarType NVar bool(* 2 species of vars*) deqnvar varcl freshv}.
+  {varclass: @VarType NVar bool(* 2 species of vars*) deqnvar varcl freshv}
+  {upnm : UpdateName NVar}.
 
 
 Notation USERVAR := true (only parsing).
@@ -461,6 +464,7 @@ Qed.
 Lemma eval_reduces_fvars :
   forall (e v : NTerm) , e ⇓ v -> subset (free_vars v) (free_vars e).
 Proof using varclass.
+  clear upnm.
   intros ? ? He. unfold closed. induction He; try auto;
   simpl in *;autorewrite with core list in *.
   (**Apply case*)
@@ -868,28 +872,70 @@ Proof using.
 Qed.
 *)
 
-Definition contVars (n:nat) : list NVar :=
-  freshVars n (Some CPSVAR) [] [].
+Definition contVars (n:nat) (suggestions : list NVar): list NVar :=
+  freshVars n (Some CPSVAR) [] suggestions.
+
+Definition mkSuggestion (s : string) : NVar :=
+updateName (nvarx, nNamed s).
+
 
 Definition contVar : NVar :=
-  nth 0 (freshVars 1 (Some CPSVAR) [] []) nvarx.
+  nth 0 (freshVars 1 (Some CPSVAR) [] [mkSuggestion "k"] ) nvarx.
    
+Lemma userVarsContVars : forall lv sugg,
+varsOfClass lv USERVAR
+-> forall n, no_repeats (contVars n sugg) /\ 
+  disjoint (contVars n sugg) lv /\ Datatypes.length (contVars n sugg) = n.
+Proof using varclass.
+  intros. unfold contVars.
+  addFreshVarsSpec.
+  dands; try tauto.
+  apply varsOfClassFreshDisjointBool.
+  assumption.
+Qed.
+
+Ltac addContVarsSpecOld  m sug H vn:=
+  let Hfr := fresh H "nr" in
+  pose proof H as Hfr;
+  apply userVarsContVars with (n:=m) (sugg:=sug) in Hfr;
+  let vf := fresh "lvcvf" in
+  remember (contVars m sug) as vf;
+  let Hdis := fresh "Hcvdis" in
+  let Hlen := fresh "Hcvlen" in
+  pose proof Hfr as  Hdis;
+  pose proof Hfr as  Hlen;
+  apply proj2, proj2 in Hlen;
+  apply proj2, proj1 in Hdis;
+  apply proj1 in Hfr;
+  simpl in Hlen;
+  dlist_len_name vf vn.
+
+Ltac addContVarsSpec  m H vn:=
+match goal with
+[H : context [contVars m ?s] |- _ ] => addContVarsSpecOld  m s H vn
+| [ |- context [contVars m ?s] ] => addContVarsSpecOld  m s H vn
+end.
+
+
+ Lemma varClassContVar : varClass contVar = false.
+Proof using.
+  intros. unfold contVar.
+  match goal with
+  [|- context [mkSuggestion ?k]] =>
+  pose proof (freshCorrect 1 (Some false) [] [mkSuggestion k]) as Hf;
+  simpl in Hf; repnd;
+  remember (freshVars 1 (Some false) [] [mkSuggestion k]) as lv
+  end.
+  dlist_len_name lv v. simpl.
+  specialize (Hf _ eq_refl v). simpl in *. auto.
+Qed.
+
 (** The inner, naive CBV CPS translation.  This introduces a lot of 
     administrative reductions, but simple things first.  Importantly,
     things that are already values are treated a little specially.  
     This ensures a substitution property 
     [cps_cvt(e{x:=v}) = (cps_cvt e){x:=(cps_vt_val v)}].
  *)
- Lemma varClassContVar : varClass contVar = false.
-Proof using.
-  intros.
-  unfold contVar.
-  pose proof (freshCorrect 1 (Some false) [] []) as Hf.
-  simpl in Hf. repnd.
-  remember (freshVars 1 (Some false) [] []) as lv.
-  dlist_len_name lv v. simpl.
-  specialize (Hf _ eq_refl v). simpl in *. auto.
-Qed.
 
 Section CPS_CVT.
 (** recursive call *)
@@ -897,7 +943,8 @@ Section CPS_CVT.
   
       (* cont \k.(ret [e1] (cont \v1.(ret [e2] (cont \v2.call v1 k v2)))) *)
   Definition cps_cvt_apply  (ce1 : CTerm) (e2: NTerm) : CTerm :=
-      let kvars := contVars 3 in 
+      let knames := ["k";"kapf";"kapArg"] in
+      let kvars := contVars 3 (map mkSuggestion knames)in 
       let k := nth 0 kvars nvarx in  
       let k1 := nth 1 kvars nvarx in  
       let k2 := nth 2 kvars nvarx in  
@@ -964,6 +1011,7 @@ End CPS_CVT.
     let kv := contVar in 
       KLam_c kv (Ret_c (vterm kv) ce).
 
+SearchAbout compose.
 Fixpoint cps_cvt (e:NTerm) {struct e}: CTerm :=
   if is_valueb e 
   then val_outer (cps_cvt_val' cps_cvt e) 
@@ -973,13 +1021,16 @@ Fixpoint cps_cvt (e:NTerm) {struct e}: CTerm :=
     | terms.oterm NApply [bterm [] e1; bterm [] e2] => 
         cps_cvt_apply cps_cvt (cps_cvt e1) e2
     | terms.oterm (NDCon d nargs) es => 
-        let kvars := contVars (S (length es)) in
+        let knames := 
+          map (mkSuggestion ∘ (fun x => append x "kdcon") ∘ nat2string10) (seq 0 (length es)) in
+        let kvars := contVars (S (length es)) ((mkSuggestion "k")::knames)in
         let k := hd nvarx kvars  in
         let tlkv := tail kvars  in
         KLam_c k (cps_cvts_chain cps_cvt tlkv es (Ret_c (vterm k)
                                                           (Con_c d (map vterm tlkv))))
     | terms.oterm (NMatch brl) ((bterm [] discriminee)::brr) => 
-      let kvars := contVars 2 in 
+      let knames := ["k";"kmd"] in
+      let kvars := contVars 2 (map mkSuggestion knames )in 
       let k := nth 0 kvars nvarx in
       let kd := nth 1 kvars nvarx in
       let brrc :=  (bterm [] (vterm kd))::(cps_cvt_branches cps_cvt (vterm k) brr) in
@@ -1144,7 +1195,7 @@ Lemma substKlam_cTrivial2 : forall x xx (b t : CTerm),
   -> closed (KLam_c x b)
   -> ssubst (KLam_c x b) [(xx,t)] = KLam_c x b.
 Proof using.
-  clear varclass.
+  clear varclass upnm.
   intros ? ? ? ? H Hb.
   change_to_ssubst_aux8;[ |simpl; rewrite H; disjoint_reasoningv; tauto].
   simpl. rewrite decide_decideP.
@@ -1190,16 +1241,7 @@ Proof using. refl. Qed.
 Definition onlyUserVars (t: NTerm) : Prop :=
   varsOfClass (all_vars t) USERVAR.
 
-Lemma userVarsContVars : forall lv,
-varsOfClass lv USERVAR
--> forall n, no_repeats (contVars n) /\ disjoint (contVars n) lv /\ Datatypes.length (contVars n) = n.
-Proof using varclass.
-  intros. unfold contVars.
-  addFreshVarsSpec.
-  dands; try tauto.
-  apply varsOfClassFreshDisjointBool.
-  assumption.
-Qed.
+
 
 Lemma userVarsContVar : forall lv,
 varsOfClass lv USERVAR
@@ -1363,21 +1405,6 @@ Proof using.
   + varsOfClassSimpl. tauto.
 Qed.
 
-Ltac addContVarsSpec  m H vn:=
-  let Hfr := fresh H "nr" in
-  pose proof H as Hfr;
-  apply userVarsContVars with (n:=m) in Hfr;
-  let vf := fresh "lvcvf" in
-  remember (contVars m) as vf;
-  let Hdis := fresh "Hcvdis" in
-  let Hlen := fresh "Hcvlen" in
-  pose proof Hfr as  Hdis;
-  pose proof Hfr as  Hlen;
-  apply proj2, proj2 in Hlen;
-  apply proj2, proj1 in Hdis;
-  apply proj1 in Hfr;
-  simpl in Hlen;
-  dlist_len_name vf vn.
 
 
 (** will be used for both the [App_e] ane [Let_e] case *)
@@ -2840,6 +2867,7 @@ Qed.
 Lemma eval_preserves_fixwf :
   forall e v, eval e v ->  fixwf e = true -> fixwf v = true.
 Proof using varclass.
+  clear evalt. clear upnm.
   intros ? ? He. induction He; intro Hfwf; try auto.
 - apply_clear IHHe3. 
   simpl in *. repeat rewrite andb_true_iff in *.
@@ -3761,12 +3789,12 @@ End TypePreservingCPS.
 *)
 End VarsOf2Class.
 
-Ltac addContVarsSpec  m H vn:=
+Ltac addContVarsSpecOld  m sug H vn:=
   let Hfr := fresh H "nr" in
   pose proof H as Hfr;
-  apply userVarsContVars with (n:=m) in Hfr;
+  apply userVarsContVars with (n:=m) (sugg:=sug) in Hfr;
   let vf := fresh "lvcvf" in
-  remember (contVars m) as vf;
+  remember (contVars m sug) as vf;
   let Hdis := fresh "Hcvdis" in
   let Hlen := fresh "Hcvlen" in
   pose proof Hfr as  Hdis;
@@ -3776,3 +3804,9 @@ Ltac addContVarsSpec  m H vn:=
   apply proj1 in Hfr;
   simpl in Hlen;
   dlist_len_name vf vn.
+
+Ltac addContVarsSpec  m H vn:=
+match goal with
+[H : context [contVars m ?s] |- _ ] => addContVarsSpecOld  m s H vn
+| [ |- context [contVars m ?s] ] => addContVarsSpecOld  m s H vn
+end.
